backend/Constpropproof.v
@@ -34,7 +34,7 @@ Require Import ValueAnalysis.
 Require Import ConstpropOp.
 Require Import Constprop.
 Require Import ConstpropOpproof.
-Require Import Linkeq.
+Require Import Linksub.
 Require Import SepcompRel.
 Require Language.
 
@@ -69,7 +69,7 @@ Lemma functions_translated:
   forall (v: val) (f: fundef),
   Genv.find_funct ge v = Some f ->
   exists sprog,
-    program_linkeq Language_RTL sprog prog /\
+    program_linksub Language_RTL sprog prog /\
     Genv.find_funct tge v = Some (transf_fundef (romem_for_program sprog) f).
 Proof.  
   intros.
@@ -83,7 +83,7 @@ Lemma function_ptr_translated:
   forall (b: block) (f: fundef),
   Genv.find_funct_ptr ge b = Some f ->
   exists sprog,
-    program_linkeq Language_RTL sprog prog /\
+    program_linksub Language_RTL sprog prog /\
     Genv.find_funct_ptr tge b = Some (transf_fundef (romem_for_program sprog) f).
 Proof.  
   intros. 
@@ -136,14 +136,14 @@ Lemma transf_ros_correct:
   find_function ge ros rs = Some f ->
   regs_lessdef rs rs' ->
   exists sprog,
-    program_linkeq Language_RTL sprog prog /\
+    program_linksub Language_RTL sprog prog /\
     find_function tge (transf_ros ae ros) rs' = Some (transf_fundef (romem_for_program sprog) f).
 Proof.
   intros until rs'; intros GE EM FF RLD. destruct ros; simpl in *.
 - (* function pointer *)
   generalize (EM r); fold (areg ae r); intro VM. generalize (RLD r); intro LD.
   assert (DEFAULT: exists sprog,
-              program_linkeq Language_RTL sprog prog /\
+              program_linksub Language_RTL sprog prog /\
               find_function tge (inl _ r) rs' = Some (transf_fundef (romem_for_program sprog) f)).
   {
     simpl. inv LD. apply functions_translated; auto. rewrite <- H0 in FF; discriminate. 
@@ -328,7 +328,7 @@ End BUILTIN_STRENGTH_REDUCTION.
 Inductive match_stackframes: stackframe -> stackframe -> Prop :=
    match_stackframe_intro:
       forall res sp pc rs f rs' sprog,
-      forall (SPROG: program_linkeq Language_RTL sprog prog),
+      forall (SPROG: program_linksub Language_RTL sprog prog),
       regs_lessdef rs rs' ->
     match_stackframes
         (Stackframe res f sp pc rs)
@@ -337,7 +337,7 @@ Inductive match_stackframes: stackframe -> stackframe -> Prop :=
 Inductive match_states: nat -> state -> state -> Prop :=
   | match_states_intro:
       forall s sp pc rs m f s' pc' rs' m' bc ae n sprog
-           (SPROG: program_linkeq Language_RTL sprog prog)
+           (SPROG: program_linksub Language_RTL sprog prog)
            (MATCH: ematch bc rs ae)
            (STACKS: list_forall2 match_stackframes s s')
            (PC: match_pc f ae n pc pc')
@@ -347,7 +347,7 @@ Inductive match_states: nat -> state -> state -> Prop :=
                     (State s' (transf_function (romem_for_program sprog) f) sp pc' rs' m')
   | match_states_call:
       forall s f args m s' args' m' sprog
-           (SPROG: program_linkeq Language_RTL sprog prog)
+           (SPROG: program_linksub Language_RTL sprog prog)
            (STACKS: list_forall2 match_stackframes s s')
            (ARGS: Val.lessdef_list args args')
            (MEM: Mem.extends m m'),
@@ -364,7 +364,7 @@ Inductive match_states: nat -> state -> state -> Prop :=
 
 Lemma match_states_succ:
   forall s f sp pc rs m s' rs' m' sprog,
-  forall (SPROG: program_linkeq Language_RTL sprog prog),
+  forall (SPROG: program_linksub Language_RTL sprog prog),
   sound_state_ext prog (State s f sp pc rs m) ->
   list_forall2 match_stackframes s s' ->
   regs_lessdef rs rs' ->
