Makefile
@@ -74,7 +74,7 @@ LIB=Axioms.v Coqlib.v Intv.v Maps.v Heaps.v Lattice.v Ordered.v \
 
 COMMON=Errors.v AST.v Events.v Globalenvs.v Memdata.v Memtype.v Memory.v \
   Values.v Smallstep.v Behaviors.v Switch.v Determinism.v Unityping.v \
-  Language.v Linkeq.v LinkerBasicproof.v LinkerProp.v SepcompRel.v Sig.v 
+  Language.v Linksub.v LinkerBasicproof.v LinkerProp.v SepcompRel.v Sig.v 
 
 # Back-end modules (in backend/, $(ARCH)/, $(ARCH)/$(VARIANT))
 
